theories/trace_index.v
@@ -12,7 +12,7 @@ Inductive ti_le : trace_index → trace_index → Prop :=
 .
 Global Instance ti_le_subseteq : SubsetEq trace_index := ti_le.
 Global Instance ti_le_rewrite : RewriteRelation (ti_le) := {}.
-Global Instance ti_le_equiv : Equiv trace_index := λ n1 n2, ti_le n1 n2 ∧ ti_le n2 n1.
+Global Instance ti_le_equiv : Equiv trace_index := λ n1 n2, n1 ⊆ n2 ∧ n2 ⊆ n1.
 
 Global Instance ti_le_preorder : PreOrder (⊆@{trace_index}).
 Proof.
@@ -71,6 +71,165 @@ Proof.
     + move => ???? IH. split. { econs. admit. } move => ?. admit.
     +
 Admitted.
+
+Lemma tiChoice_mono T f1 f2:
+  (∀ x, f1 x ⊆ f2 x) →
+  tiChoice T f1 ⊆ tiChoice T f2.
+Proof. move => ?. econs. econs. naive_solver. Qed.
+
+Fixpoint ti_min (n1 : trace_index) : trace_index → trace_index :=
+  fix go n2 :=
+  match n1, n2 with
+  | tiChoice T f, _ => tiChoice T (λ x, ti_min (f x) n2)
+  | _, tiChoice T f => tiChoice T (λ x, go (f x))
+  | tiO, _ => tiO
+  | _, tiO => tiO
+  | tiS n1', tiS n2' => tiS (ti_min n1' n2')
+  end.
+
+Lemma ti_min_choice_l_1 T f n :
+  tiChoice T (λ x, ti_min (f x) n) ⊆ ti_min (tiChoice T f) n.
+Proof. by destruct n. Qed.
+Lemma ti_min_choice_l_2 T f n :
+  ti_min (tiChoice T f) n ⊆ tiChoice T (λ x, ti_min (f x) n).
+Proof. by destruct n. Qed.
+
+Lemma ti_min_choice_r_1 T f n :
+  tiChoice T (λ x, ti_min n (f x)) ⊆ ti_min n (tiChoice T f).
+Proof.
+  elim: n => //=.
+  move => T' f' IH. econs => x.
+  destruct (f x) eqn: Hx => //=; econs => ?; rewrite -Hx.
+  all: econs; (etrans; [|by apply: IH]); by econs.
+Qed.
+
+Lemma ti_min_choice_r_2 T f n :
+  ti_min n (tiChoice T f) ⊆ tiChoice T (λ x, ti_min n (f x)).
+Proof.
+  elim: n => //=.
+  move => T' f' IH. econs => x'. etrans; [apply: IH|].
+  apply tiChoice_mono => x.
+  by destruct (f x) eqn: Hx => //=; rewrite -Hx; econs.
+Qed.
+
+Lemma ti_min_mono n m n' m':
+  n ⊆ n' →
+  m ⊆ m' →
+  ti_min n m ⊆ ti_min n' m'.
+Proof.
+  move => Hn. elim: Hn m m' => /=; clear.
+  - move => n m m' Hm. elim: Hm n => //=; clear.
+    + econs.
+    + econs.
+    + move => ???? IH ?. econs => ?. apply: IH.
+    + move => ????? IH ?. rewrite -ti_min_choice_r_1. econs. apply: IH.
+  - move => n1 n2 _ IH m m' Hm. elim: Hm.
+    + econs.
+    + econs. by apply: IH.
+    + move => ???? IH2. econs => ?. apply: IH2.
+    + move => ????? IH2. econs. apply: IH2.
+  - move => T f n ? IH m m' Hm. destruct m; econs => ?; by apply: IH.
+  - move => T f n x ? IH m m' Hm. destruct m'; econs; by apply: IH.
+Qed.
+
+Global Instance ti_mono_proper :
+  Proper ((⊆) ==> (⊆) ==> (⊆)) ti_min.
+Proof. move => ??????. by apply: ti_min_mono. Qed.
+Global Instance ti_mono_flip_proper :
+  Proper (flip (⊆) ==> flip (⊆) ==> flip (⊆)) ti_min.
+Proof. move => ??????. by apply: ti_min_mono. Qed.
+Global Instance ti_mono_equiv_proper :
+  Proper ((≡) ==> (≡) ==> (≡)) ti_min.
+Proof. move => ?? [Hn1 Hn2] ?? [Hm1 Hm2]. split; by apply: ti_min_mono. Qed.
+
+Lemma ti_min_comm_1 n m:
+  ti_min n m ⊆ ti_min m n.
+Proof.
+  elim: n m => /=.
+  - elim => //= ?? IH. apply tiChoice_mono => ?. apply: IH.
+  - move => n IH m.
+    elim: m.
+    + econs.
+    + move => ??. econs. apply: IH.
+    + move => ?? IH2. apply tiChoice_mono => ?. apply: IH2.
+  - move => ?? IH m. rewrite -ti_min_choice_r_1.
+    destruct m; apply tiChoice_mono => ?; apply: IH.
+Qed.
+
+Lemma ti_min_comm n m:
+  ti_min n m ≡ ti_min m n.
+Proof. split; apply ti_min_comm_1. Qed.
+
+Lemma ti_min_assoc_1 n m p:
+  ti_min n (ti_min m p) ⊆ ti_min (ti_min n m) p.
+Proof.
+  elim: n m p.
+  - simpl. elim => //=.
+    + elim => // ?? IH. apply tiChoice_mono => ?. apply: IH.
+    + move => n IH. elim => // ?? IH2. apply tiChoice_mono => ?. apply: IH2.
+    + move => T f IH. case => *; apply tiChoice_mono => ?; apply: IH.
+  - move => n IH m /=.
+    elim: m.
+    + elim => //= ?? IH2. apply tiChoice_mono => ?; apply: IH2.
+    + move => m IH2.
+      elim => //= *.
+      * econs. apply: IH.
+      * apply tiChoice_mono => ?; naive_solver.
+    + move => T f IH2 /= p. destruct p; apply tiChoice_mono => ?; apply: IH2.
+  - move => T f IH m p. rewrite !ti_min_choice_l_2. rewrite -!ti_min_choice_l_1.
+    by apply tiChoice_mono => ?.
+Qed.
+
+Lemma ti_min_assoc_2 n m p:
+  ti_min (ti_min n m) p ⊆ ti_min n (ti_min m p).
+Proof. by rewrite (ti_min_comm_1 n m) ti_min_comm_1 ti_min_assoc_1 (ti_min_comm_1 p m) ti_min_comm_1. Qed.
+
+Lemma ti_min_assoc n m p:
+  ti_min n (ti_min m p) ≡ ti_min (ti_min n m) p.
+Proof. split; [apply ti_min_assoc_1 | apply ti_min_assoc_2 ]. Qed.
+
+Lemma ti_min_le_l n m:
+  ti_min n m ⊆ n.
+Proof.
+  elim: n m => /=.
+  - elim => // ?? IH. econs => ?. apply: IH.
+  - move => n IH m.
+    elim: m.
+    + econs.
+    + move => ??. econs. apply: IH.
+    + move => ?? IH2. econs => ?. apply: IH2.
+  - move => ?? IH m. destruct m; econs => ?; econs; apply: IH.
+Qed.
+
+Lemma ti_min_le_r n m:
+  ti_min n m ⊆ m.
+Proof. etrans; [apply ti_min_comm_1|]. apply ti_min_le_l. Qed.
+
+Lemma ti_min_l_2 n m:
+  n ⊆ m → n ⊆ ti_min n m.
+Proof.
+  elim => /=; clear.
+  - econs.
+  - move => ????. by econs.
+  - move => ?? m ? IH. econs => ?. destruct m; econs; apply: IH.
+  - move => ?? n ?? IH. rewrite -ti_min_choice_r_1. by econs.
+Qed.
+
+Lemma ti_min_l n m:
+  n ⊆ m → ti_min n m ≡ n.
+Proof. move => Hn. split; [apply ti_min_le_l | by apply ti_min_l_2]. Qed.
+
+Lemma ti_min_r_2 n m:
+  m ⊆ n → m ⊆ ti_min n m.
+Proof. move => ?. etrans; [by apply ti_min_l_2|]. apply ti_min_comm. Qed.
+
+Lemma ti_min_r n m:
+  m ⊆ n → ti_min n m ≡ m.
+Proof. move => Hn. split; [apply ti_min_le_r | by apply ti_min_r_2]. Qed.
+
+Lemma ti_min_id n:
+  ti_min n n ≡ n.
+Proof. by apply ti_min_l. Qed.
 
 Lemma ti_lt_impl_le (n1 n2 : trace_index):
   n1 ⊂ n2 →
